# Week 2 - Lab Sheet

```agda
{-# OPTIONS --without-K --safe #-}
module Pool.Lab.lab2 where

open import prelude hiding (if_then_else_;_||_)
```

## Part I: Booleans

### Section 1: Operations on Booleans

#### Exercise 1.1

We have already defined `if-then-else` like so:

```agda
if_then_else_ : {A : Type} → Bool → A → A → A
if true  then x else y = x
if false then x else y = y
```

But this requires our two branches to be of the same type A. Instead, we could
define `if-then-else` to have branches of different types, using the `Either`
datatype

```agda
data Either (A B : Type) : Type where
 left  : A → Either A B
 right : B → Either A B

if'_then_else_ : {A B : Type} → Bool → A → B → Either A B
if' b then x else y = {!!}
```

**Define** this function.

#### Exercise 1.2

We can define the `_||_` function in (at least) two different ways, depending on
how much pattern-matching we wish to perform:

```agda
_||_ : Bool → Bool → Bool
true  || y = {!!}
false || y = {!!}

_||'_ : Bool → Bool → Bool
true  ||' true  = {!!}
true  ||' false = {!!}
false ||' true  = {!!}
false ||' false = {!!}
```

**Complete** the two holes for `_||_` and the four holes for `_||'_`.

The `_||_` operator is *associative*, meaning `a || (b || c) ≡ (a || b) || c`.

We can prove this for both of our definitions:

```agda
||-assoc : (a b c : Bool)  → a ||  (b ||  c) ≡ (a ||  b) || c
||-assoc a b c = {!!}

||'-assoc : (a b c : Bool) → a ||' (b ||' c) ≡ (a ||' b) ||' c
||'-assoc a b c = {!!}
```

**Complete** both of these proofs.
(Hint: Because `||` was defined by pattern matching on the first argument, it
may be helpful to use the same strategy.)

Which of these did you prefer proving, and why?

#### Exercise 1.3

**Complete** the proof that Boolean disjunction is commutative:

```agda
||-is-commutative : (a b : Bool) → a || b ≡ b || a
||-is-commutative a b = {!!}
```

#### Exercise 1.4

**Complete** the proof that `false` is the left unit element of `||`:

```agda
false-left-unit-for-|| : (b : Bool) → false || b ≡ b
false-left-unit-for-|| b = {!!}
```

**Complete** the proof that `false` is the right unit element of `||`:

```agda
false-right-unit-for-|| : (b : Bool) → b || false ≡ b
false-right-unit-for-|| b = {!!}
```

#### Exercise 1.5

Now prove the analogous properties for `&&`.

**Complete** the proof that Boolean conjunction is associative:

```agda
&&-is-associative : (a b c : Bool) → a && (b && c) ≡ (a && b) && c
&&-is-associative a b c = {!!}
```

**Complete** the proof that Boolean conjunction is commutative:

```agda
&&-is-commutative : (a b : Bool) → a && b ≡ b && a
&&-is-commutative a b = {!!}
```

**Complete** the proof that that `true` is the left unit element of `&&`:

```agda
true-left-unit-for-&& : (b : Bool) → true && b ≡ b
true-left-unit-for-&& b = {!!}
```

**Complete** the proof that that `true` is the right unit element of `&&`:

```agda
true-right-unit-for-&& : (b : Bool) → b && true ≡ b
true-right-unit-for-&& b = {!!}
```

#### Exercise 1.6

An important algebraic property between two operators is *distributivity*. For
example, multiplication distributes over addition since `x * (y + z) = (x * y) +
(x * z)` for every `x, y, z ∈ ℕ`. The same is the case for the Boolean
conjunction and disjunction operators we have defined.

**Complete** the proof that Boolean conjunction distributes over Boolean
disjunction:

```agda
&&-distributes-over-|| : (a b c : Bool) → a && (b || c) ≡ (a && b) || (a && c)
&&-distributes-over-|| a b c = {!!}
```

```agda
||-distributes-over-&& : (a b c : Bool) → a || (b && c) ≡ (a || b) && (a || c)
||-distributes-over-&& a b c = {!!}
```


### Section 2: Identity type and `Bool`

With these exercises, you will practise with the identity type and `Bool`.

#### Exercise 2.1

Recall how we defined `_≣_` for [natural
numbers](../introduction.lagda.md#the-empty-type-and-the-unit-type). We could do
the same for the Booleans.

```agda
_≣_ : Bool → Bool → Type
x ≣ y = {!!}
```

**Define** this function.

Tip: you can type `≣` as `\===`.

#### Exercise 2.2

We can also define a Boolean-valued equality function.

```agda
_==_ : Bool → Bool → Bool
x == y = {!!}
```

**Define** this function.

#### Exercise 2.3

Now we write a conversion function from `x ≡ y` to `x ≣ y`, just like the
function `back` in
[introduction](../introduction.lagda.md#the-identity-type-former-__).

```agda
≡-to-≣ : (x y : Bool) → x ≡ y → x ≣ y
≡-to-≣ x y e = {!!}
```

**Complete** this function.

#### Exercise 2.4

The following helper function makes some functions nicer to read.

```agda
is-true : Bool → Type
is-true b = b ≡ true
```

Now we can consider another conversion function.

```agda
≣-to-== : (x y : Bool) → x ≣ y → is-true (x == y)
≣-to-== x y e = {!!}
```

**Define** this function.

#### Exercise 2.5

And similarly, we have

```agda
==-to-≡ : (x y : Bool) → is-true (x == y) → x ≡ y
==-to-≡ x y e = {!!}
```

**Define** this function.

#### Exercise 2.6

Finally, we can use the above functions to define the three remaining
implications

```agda
≡-to-== : (x y : Bool) → x ≡ y → is-true (x == y)
≡-to-== x y e = {!!}

≣-to-≡ : (x y : Bool) → x ≣ y → x ≡ y
≣-to-≡ x y e = {!!}

==-to-≣ : (x y : Bool) → is-true (x == y) → x ≣ y
==-to-≣ x y e = {!!}
```

**Complete** these functions.


## Part II: Natural numbers

### Section 1: Some functions on natural numbers

#### Exercise 1.1

**Complete** the proof of the fact that `(suc x) + y ≡ suc (x + y)`

```agda
+-suc-on-left : (x y : ℕ) → (suc x) + y ≡ suc (x + y)
+-suc-on-left x y = {!!}
```

#### Exercise 1.2

We can define `max` operation on natural numbers as follows:

```agda
max : ℕ → ℕ → ℕ
max zero    n       = n
max (suc m) zero    = suc m
max (suc m) (suc n) = suc (max m n)
```

**Define** the function `min` analogously:

```agda
min : ℕ → ℕ → ℕ
min m n = {!!}
```

### Section 2: Natural numbers and proofs using induction

The function `+-0-on-right` expresses the fact that `0` is a right unit of the
operation `_+_`. Notice how we use an inductive hypothesis (the recursive call)
in the proof. (Spelling this out, `IH` tells us that `x + 0 ≡ x`, so that `ap
suc IH` witnesses that `suc (x + 0) ≡ suc x`.)

```agda
+-0-on-right : (x : ℕ) → x + 0 ≡ x
+-0-on-right zero    = refl zero
+-0-on-right (suc x) = ap suc IH
 where
  IH : x + 0 ≡ x -- IH is short for induction hypothesis
  IH = +-0-on-right x
```

Using similar induction hypotheses, try to complete the following exercises.


#### Exercise 2.1

**Complete** the proof:

```agda
+-suc-on-right : (x y : ℕ) → x + suc y ≡ suc (x + y)
+-suc-on-right x y = {!!}
```

#### Exercise 2.2

In algebra, an operator `_*_` is called idempotent iff `x * x = x` for every
`x`. `max` is an example of an idempotent operator:

**Complete** the hole to prove that `max` is idempotent:

```agda
max-idempotent : (x : ℕ) → max x x ≡ x
max-idempotent x = {!!}
```

#### Exercise 2.3

**Complete** the hole by constructing a proof of the fact that `max` is a
commutative operator:

```agda
max-commutative : (x y : ℕ) → max x y ≡ max y x
max-commutative x y = {!!}
```

#### Exercise 2.4

Now recall that we defined `min` in Exercise 1.2. Similarly, we can show that
`min` is idempotent and commutative too.

**Complete** the proof that `min` is idempotent:

```agda
min-idempotent : (x : ℕ) → min x x ≡ x
min-idempotent x = {!!}
```

#### Exercise 2.5

**Complete** the proof that `min` is commutative:

```agda
min-commutative : (x y : ℕ) → min x y ≡ min y x
min-commutative x y = {!!}
```
