# Week 5 - Lab Sheet

```agda
{-# OPTIONS --without-K --safe #-}

module Pool.Lab.lab5 where

open import prelude
open import natural-numbers-functions hiding (_‚â§_ ; is-even ; is-odd ; +-comm)
open import List-functions
open import isomorphisms
```

We will also want to use some things from the Lab and Homework sheet of Week 4:

```agda
open import Pool.Homework.homework4-solutions
open import Pool.Lab.lab4-solutions
```

## Part I: Length

In the file [List-functions.lagda.md](../List-functions.lagda.md), the
function `length` is recursively defined as follows.

```agdacode
length : {A : Type} ‚Üí List A ‚Üí ‚Ñï
length []        = 0
length (x :: xs) = 1 + length xs
```

In the following exercises we will prove some facts involving the length of
lists. In doing so, you will practise with inductive proofs.

### Exercise 1.1

Recall that we defined `map` as follows (see
[List-functions.lagda.md](../List-functions.lagda.md)).

```agdacode
map : {A B : Type} ‚Üí (A ‚Üí B) ‚Üí List A ‚Üí List B
map f []        = []
map f (x :: xs) = f x :: map f xs
```

**Prove** that `map` preserves the length of a list.

```agda
map-preserves-length : {A B : Type} (f : A ‚Üí B) (xs : List A)
                     ‚Üí length (map f xs) ‚â° length xs
map-preserves-length = {!!}
```

### Exercise 1.2

Another useful fact is that the length of two concatenated lists is the sum of
their respective lengths. **Complete** the proof of this fact.

```agda
length-of-++ : {A : Type} (xs ys : List A)
             ‚Üí length (xs ++ ys) ‚â° length xs + length ys
length-of-++ = {!!}
```

### Exercise 1.3

Recall `‚â§'` from Lab Sheet 4 and `‚âº'` from Homework Sheet 4

```agdacode
_‚â§'_ : ‚Ñï ‚Üí ‚Ñï ‚Üí Type
x ‚â§' y = Œ£ k Íûâ ‚Ñï , x + k ‚â° y
```

```agdacode
_‚âº'_ : {X : Type} ‚Üí List X ‚Üí List X ‚Üí Type
_‚âº'_ {X} xs ys = Œ£ zs Íûâ List X , xs ++ zs ‚â° ys
```

and that `x ‚â§' y` expresses that the natural number `x` is less than or equal to
the natural number `y`, while `xs ‚âº' ys` expresses that the list `xs` is a
prefix of the list `ys`.

**Prove** that the length of a prefix of a list `ys` is less than the length of
`ys`, relating the two notions above.

```agda
length-of-prefix : {A : Type} (xs ys : List A)
                 ‚Üí xs ‚âº' ys
                 ‚Üí length xs ‚â§' length ys
length-of-prefix = {!!}
```

### Exercise 1.4

A nice use case of the length function is that we are now able to define safe
`head` and `tail` operations on nonempty lists.

We say that a list is *nonempty* if its length is at least 1.
```agda
is-nonempty : {A : Type} ‚Üí List A ‚Üí Type
is-nonempty xs = 1 ‚â§' length xs
```

We can then define `tail` as follows.
```agda
tail : {A : Type} (xs : List A) ‚Üí is-nonempty xs ‚Üí List A
tail (x :: xs) p = xs
```

Agda accepts this definition and does not complain about missing the `[]`-case,
because it realizes that `[]` does not satisfy `is-nonempty`.

#### Exercise 1.4a

```agda
head : {A : Type} (xs : List A) ‚Üí is-nonempty xs ‚Üí A
head = {!!}
```

**Complete** the definition of `head` yourself.

#### Exercise 1.4b

```agda
length-of-tail : {A : Type} (xs : List A) (p : 1 ‚â§' length xs)
               ‚Üí 1 + length (tail xs p) ‚â° length xs
length-of-tail = {!!}
```

**Prove** that the length of a list is obtained by adding 1 to the length of the
tail.

#### Exercise 1.4c

```agda
‚â§'-suc-lemma : (n : ‚Ñï) ‚Üí n ‚â§' (1 + n)
‚â§'-suc-lemma = {!!}

length-of-tail-decreases : {A : Type} (xs : List A) (p : 1 ‚â§' length xs)
                         ‚Üí length (tail xs p) ‚â§' length xs
length-of-tail-decreases = {!!}
```

**Complete** the proof of the following lemma and use it to prove that the
length of the tail of a list is less than the length of the full list.

## Part II: Isomorphisms

Make sure you have read the [file on isomorphisms](../isomorphisms.lagda.md),
where we define ismorphisms and show that `Bool ‚âÖ ùüö`.

You will now give three more isomorphisms. In each case, you should think
about *why* and *how* each pair of types are isomorphic before attemping to
formalise the isomorphism.

### Exercise 2.1

```agda
√ó-iso : (X Y : Type) ‚Üí X √ó Y ‚âÖ Y √ó X
√ó-iso X Y = record { bijection = f ; bijectivity = f-is-bijection }
 where
  f : X √ó Y ‚Üí Y √ó X
  f = {!!}

  g : Y √ó X ‚Üí X √ó Y
  g = {!!}

  gf : g ‚àò f ‚àº id
  gf = {!!}

  fg : f ‚àò g ‚àº id
  fg = {!!}

  f-is-bijection : is-bijection f
  f-is-bijection = record { inverse = g ; Œ∑ = gf ; Œµ = fg }
```

**Show** that X √ó Y is isomorphic to Y √ó X using the above template.

### Exercise 2.2

```agda
+-iso : (X Y : Type) ‚Üí X ‚àî Y ‚âÖ Y ‚àî X
+-iso X Y = record { bijection = f ; bijectivity = f-is-bijection }
 where
  f : X ‚àî Y ‚Üí Y ‚àî X
  f = {!!}

  g : Y ‚àî X ‚Üí X ‚àî Y
  g = {!!}

  gf : g ‚àò f ‚àº id
  gf = {!!}

  fg : f ‚àò g ‚àº id
  fg = {!!}

  f-is-bijection : is-bijection f
  f-is-bijection = record { inverse = g ; Œ∑ = gf ; Œµ = fg }
```

### Exercise 2.3

```agda
lists-from-vectors : {A : Type} ‚Üí List A ‚âÖ (Œ£ n Íûâ ‚Ñï , Vector A n)
lists-from-vectors {A}
 = record { bijection = f ; bijectivity = f-is-bijection }
 where
  f : List A ‚Üí Œ£ n Íûâ ‚Ñï , Vector A n
  f = {!!}

  g : Œ£ n Íûâ ‚Ñï , Vector A n ‚Üí List A
  g = {!!}

  gf : g ‚àò f ‚àº id
  gf = {!!}

  fg : f ‚àò g ‚àº id
  fg = {!!}

  f-is-bijection : is-bijection f
  f-is-bijection = record { inverse = g ; Œ∑ = gf ; Œµ = fg }
```

**Show** that the the type `List A` is isomorphic to the type `Œ£ (Vector A)`.

(Note that this is the first question in [this question
sheet](../vector-and-list-isomorphisms.lagda.md)).

Hint: The statement of Exercise 2.3b may help you.

### Exercise 2.3b

```agda
open _‚âÖ_

lfv-preserves-length : {A : Type} (xs : List A)
                     ‚Üí fst (bijection lists-from-vectors xs)
                     ‚â° length xs
lfv-preserves-length = {!!}
```

Notice how `bijection` extracts the function `f` you defined in
`lists-from-vectors`.

**Prove** that for any `xs : List A`, the length of `xs` is the same as the
first projection of `f xs : Œ£ (Vector A)` (where `f : ‚Ñï ‚Üí List ùüô` is as you
defined in Exercise 4a).

## Part III: Evenness

In the lecture notes, you have seen the predicates `is-even` and `is-odd`:

```agda
is-even is-odd : ‚Ñï ‚Üí Type
is-even x = Œ£ y Íûâ ‚Ñï , x ‚â° 2 * y
is-odd  x = Œ£ y Íûâ ‚Ñï , x ‚â° 1 + 2 * y
```

In these exercises, we will define a Boolean-valued version of the `is-even`
predicate and prove that the two versions are _logically_ equivalent:

```agda
check-even : ‚Ñï ‚Üí Bool
check-even zero          = true
check-even (suc zero)    = false
check-even (suc (suc n)) = check-even n
```

### Exercise 3.1

First, we will have to prove two lemmas that we will use in Exercise 3.2, where
we will prove our main result.

```agda
evenness-lemma‚ÇÅ : (n : ‚Ñï) ‚Üí is-even (2 + n) ‚Üí is-even n
evenness-lemma‚ÇÅ n (suc k , p) = k , goal
 where
  subgoal : suc (suc n) ‚â° suc (suc (2 * k))
  subgoal = suc (suc n)       ‚â°‚ü® {!!} ‚ü©
            suc k + suc k     ‚â°‚ü® {!!} ‚ü©
            suc ((suc k) + k) ‚àé

  goal : n ‚â° 2 * k
  goal = suc-is-injective (suc-is-injective subgoal)

evenness-lemma‚ÇÇ : (n : ‚Ñï) ‚Üí is-even n ‚Üí is-even (2 + n)
evenness-lemma‚ÇÇ n (k , p) = suc k , goal
 where
  goal : 2 + n ‚â° 2 * suc k
  goal = 2 + n         ‚â°‚ü® {!!} ‚ü©
         2 + (k + k)   ‚â°‚ü® {!!} ‚ü©
         suc k + suc k ‚àé
```

**Complete** the above proofs.

### Exercise 3.2

**Prove** that if `is-even n` is inhabited, then `check-even n ‚â° true`.

```agda
even‚áícheck-even : (n : ‚Ñï) ‚Üí is-even n ‚Üí check-even n ‚â° true
even‚áícheck-even = {!!}
```

**Prove** that if `check-even n ‚â° true` then `is-even n` is inhabited:

```agda
check-even‚áíeven : (n : ‚Ñï) ‚Üí check-even n ‚â° true ‚Üí is-even n
check-even‚áíeven = {!!}
```
