
Martin Escardo.
Notes originally written for the module "Advanced Functional Programming"
at the School of Computer Science of the University of Birmingham, UK.


<!--
```agda
{-# OPTIONS --without-K --safe #-}

module natural-numbers-functions where


open import prelude
open import negation
```
-->
# Natural numbers functions, relations and properties

## Some general properties

```agda
suc-is-not-zero : {x : ‚Ñï} ‚Üí suc x ‚â¢ 0
suc-is-not-zero ()

zero-is-not-suc : {x : ‚Ñï} ‚Üí 0 ‚â¢ suc x
zero-is-not-suc ()

pred : ‚Ñï ‚Üí ‚Ñï
pred 0       = 0
pred (suc n) = n

suc-is-injective : {x y : ‚Ñï} ‚Üí suc x ‚â° suc y ‚Üí x ‚â° y
suc-is-injective = ap pred
```

## Order relation _‚â§_

The less-than order on natural numbers can be defined in a number of
equivalent ways. The first one says that `x ‚â§ y` iff `x + z ‚â° y` for
some `z`:
```agda
_‚â§‚ÇÄ_ : ‚Ñï ‚Üí ‚Ñï ‚Üí Type
x ‚â§‚ÇÄ y = Œ£ a Íûâ ‚Ñï , x + a ‚â° y
```
The second one is defined by recursion:
```agda
_‚â§‚ÇÅ_ : ‚Ñï ‚Üí ‚Ñï ‚Üí Type
0     ‚â§‚ÇÅ y     = ùüô
suc x ‚â§‚ÇÅ 0     = ùüò
suc x ‚â§‚ÇÅ suc y = x ‚â§‚ÇÅ y
```
The third one, which we will as the official one, is defined *by induction* using `data`:
```agda
data _‚â§_ : ‚Ñï ‚Üí ‚Ñï ‚Üí Type where
 0-smallest      : {y : ‚Ñï} ‚Üí 0 ‚â§ y
 suc-preserves-‚â§ : {x y : ‚Ñï} ‚Üí x ‚â§ y ‚Üí suc x ‚â§ suc y

_‚â•_ : ‚Ñï ‚Üí ‚Ñï ‚Üí Type
x ‚â• y = y ‚â§ x

infix 0 _‚â§_
infix 0 _‚â•_
```

We will now show some properties of these relations.
```agda
suc-reflects-‚â§ : {x y : ‚Ñï} ‚Üí suc x ‚â§ suc y ‚Üí x ‚â§ y
suc-reflects-‚â§ {x} {y} (suc-preserves-‚â§ l) = l

suc-preserves-‚â§‚ÇÄ : {x y : ‚Ñï} ‚Üí x ‚â§‚ÇÄ y ‚Üí suc x ‚â§‚ÇÄ suc y
suc-preserves-‚â§‚ÇÄ {x} {y} (a , p) = Œ≥
 where
  q : suc (x + a) ‚â° suc y
  q = ap suc p

  Œ≥ : suc x ‚â§‚ÇÄ suc y
  Œ≥ = (a , q)

‚â§‚ÇÄ-implies-‚â§‚ÇÅ : {x y : ‚Ñï} ‚Üí x ‚â§‚ÇÄ y ‚Üí x ‚â§‚ÇÅ y
‚â§‚ÇÄ-implies-‚â§‚ÇÅ {zero}  {y}     (a , p) = ‚ãÜ
‚â§‚ÇÄ-implies-‚â§‚ÇÅ {suc x} {suc y} (a , p) = IH
 where
  q : x + a ‚â° y
  q = suc-is-injective p

  Œ≥ : x ‚â§‚ÇÄ y
  Œ≥ = (a , q)

  IH : x ‚â§‚ÇÅ y
  IH = ‚â§‚ÇÄ-implies-‚â§‚ÇÅ {x} {y} Œ≥

‚â§‚ÇÅ-implies-‚â§ : {x y : ‚Ñï} ‚Üí x ‚â§‚ÇÅ y ‚Üí x ‚â§ y
‚â§‚ÇÅ-implies-‚â§ {zero}  {y}     l = 0-smallest
‚â§‚ÇÅ-implies-‚â§ {suc x} {suc y} l = Œ≥
 where
  IH : x ‚â§ y
  IH = ‚â§‚ÇÅ-implies-‚â§ l

  Œ≥ : suc x ‚â§ suc y
  Œ≥ = suc-preserves-‚â§ IH

‚â§-implies-‚â§‚ÇÄ : {x y : ‚Ñï} ‚Üí x ‚â§ y ‚Üí x ‚â§‚ÇÄ y
‚â§-implies-‚â§‚ÇÄ {0}     {y}      0-smallest         = (y , refl y)
‚â§-implies-‚â§‚ÇÄ {suc x} {suc y} (suc-preserves-‚â§ l) = Œ≥
 where
  IH : x ‚â§‚ÇÄ y
  IH = ‚â§-implies-‚â§‚ÇÄ {x} {y} l

  Œ≥ : suc x ‚â§‚ÇÄ suc y
  Œ≥ = suc-preserves-‚â§‚ÇÄ IH
```

## Exponential function

```agda
_^_ : ‚Ñï ‚Üí ‚Ñï ‚Üí ‚Ñï
y ^ 0     = 1
y ^ suc x = y * y ^ x

infix 40 _^_
```

## Maximum and minimum

```agda
max : ‚Ñï ‚Üí ‚Ñï ‚Üí ‚Ñï
max 0       y       = y
max (suc x) 0       = suc x
max (suc x) (suc y) = suc (max x y)

min : ‚Ñï ‚Üí ‚Ñï ‚Üí ‚Ñï
min 0       y       = 0
min (suc x) 0       = 0
min (suc x) (suc y) = suc (min x y)
```

## No natural number is its own successo

We now show that there is no natural number `x` such that `x = suc x`.
```agda
every-number-is-not-its-own-successor : (x : ‚Ñï) ‚Üí x ‚â¢ suc x
every-number-is-not-its-own-successor 0       e = zero-is-not-suc e
every-number-is-not-its-own-successor (suc x) e = goal
 where
  IH : x ‚â¢ suc x
  IH = every-number-is-not-its-own-successor x

  e' : x ‚â° suc x
  e' = suc-is-injective e

  goal : ùüò
  goal = IH e'

there-is-no-number-which-is-its-own-successor : ¬¨ (Œ£ x Íûâ ‚Ñï , x ‚â° suc x)
there-is-no-number-which-is-its-own-successor (x , e) = every-number-is-not-its-own-successor x e
```

## Prime numbers

```agda
is-prime : ‚Ñï ‚Üí Type
is-prime n = (n ‚â• 2) √ó ((x y : ‚Ñï) ‚Üí x * y ‚â° n ‚Üí (x ‚â° 1) ‚àî (x ‚â° n))
```
**Exercise.** Show that `is-prime n` is [decidable](decidability.lagda.md) for every `n : ‚Ñï`. Hard.

The following is a conjecture that so far mathematicians haven't been able to prove or disprove. But we can still say what the conjecture is in Agda:
```agda
twin-prime-conjecture : Type
twin-prime-conjecture = (n : ‚Ñï) ‚Üí Œ£ p Íûâ ‚Ñï , (p ‚â• n)
                                          √ó is-prime p
                                          √ó is-prime (p + 2)
```

## Properties of addition

```agda
+-base : (x : ‚Ñï) ‚Üí x + 0 ‚â° x
+-base 0       = 0 + 0       ‚â°‚ü® refl _ ‚ü©
                 0           ‚àé

+-base (suc x) = suc (x + 0) ‚â°‚ü® ap suc (+-base x) ‚ü©
                 suc x       ‚àé

+-step : (x y : ‚Ñï) ‚Üí x + suc y ‚â° suc (x + y)
+-step 0       y = 0 + suc y         ‚â°‚ü® refl _ ‚ü©
                   suc y             ‚àé

+-step (suc x) y = suc x + suc y     ‚â°‚ü® refl _ ‚ü©
                   suc (x + suc y)   ‚â°‚ü® ap suc (+-step x y) ‚ü©
                   suc (suc (x + y)) ‚â°‚ü® refl _ ‚ü©
                   suc (suc x + y)   ‚àé

+-comm : (x y : ‚Ñï) ‚Üí x + y ‚â° y + x
+-comm 0       y = 0 + y       ‚â°‚ü® refl _ ‚ü©
                   y           ‚â°‚ü® sym (+-base y) ‚ü©
                   y + 0       ‚àé

+-comm (suc x) y = suc x + y   ‚â°‚ü® refl _ ‚ü©
                          suc (x + y) ‚â°‚ü® ap suc (+-comm x y) ‚ü©
                          suc (y + x) ‚â°‚ü® refl _ ‚ü©
                          suc y + x   ‚â°‚ü® sym (+-step y x) ‚ü©
                          y + suc x   ‚àé
```

## Associativity of addition

```agda
+-assoc : (x y z : ‚Ñï) ‚Üí (x + y) + z ‚â° x + (y + z)
+-assoc 0       y z = refl (y + z)
+-assoc (suc x) y z =
   (suc x + y) + z   ‚â°‚ü® refl _ ‚ü©
   suc (x + y) + z   ‚â°‚ü® refl _ ‚ü©
   suc ((x + y) + z) ‚â°‚ü® ap suc (+-assoc x y z) ‚ü©
   suc (x + (y + z)) ‚â°‚ü® refl _ ‚ü©
   suc x + (y + z)   ‚àé

+-assoc' : (x y z : ‚Ñï) ‚Üí (x + y) + z ‚â° x + (y + z)
+-assoc' 0       y z = refl (y + z)
+-assoc' (suc x) y z = ap suc (+-assoc' x y z)
```

## 1 is a neutral element of multiplication

```agda
1-*-left-neutral : (x : ‚Ñï) ‚Üí 1 * x ‚â° x
1-*-left-neutral x = refl x

1-*-right-neutral : (x : ‚Ñï) ‚Üí x * 1 ‚â° x
1-*-right-neutral 0       = refl 0
1-*-right-neutral (suc x) =
   suc x * 1 ‚â°‚ü® refl _ ‚ü©
   x * 1 + 1 ‚â°‚ü® ap (_+ 1) (1-*-right-neutral x) ‚ü©
   x + 1     ‚â°‚ü® +-comm x 1 ‚ü©
   1 + x     ‚â°‚ü® refl _ ‚ü©
   suc x     ‚àé
```

## Multiplication distributes over addition:

```agda
*-+-distrib : (x y z : ‚Ñï) ‚Üí x * (y + z) ‚â° x * y + x * z
*-+-distrib 0       y z = refl 0
*-+-distrib (suc x) y z = goal
 where
  IH : x * (y + z) ‚â° x * y + x * z
  IH = *-+-distrib x y z

  goal : suc x * (y + z) ‚â° suc x * y + suc x * z
  goal = suc x * (y + z)         ‚â°‚ü® refl _ ‚ü©
         x * (y + z) + (y + z)   ‚â°‚ü® ap (_+ y + z) IH ‚ü©
         (x * y + x * z) + y + z ‚â°‚ü® +-assoc (x * y) (x * z) (y + z) ‚ü©
         x * y + x * z + y + z   ‚â°‚ü® ap (x * y +_) (sym (+-assoc (x * z) y z)) ‚ü©
         x * y + (x * z + y) + z ‚â°‚ü® ap (Œª - ‚Üí x * y + - + z) (+-comm (x * z) y) ‚ü©
         x * y + (y + x * z) + z ‚â°‚ü® ap (x * y +_) (+-assoc y (x * z) z) ‚ü©
         x * y + y + x * z + z   ‚â°‚ü® sym (+-assoc (x * y) y (x * z + z)) ‚ü©
         (x * y + y) + x * z + z ‚â°‚ü® refl _ ‚ü©
         suc x * y + suc x * z   ‚àé
```

## Commutativity of multiplication

```agda
*-base : (x : ‚Ñï) ‚Üí x * 0 ‚â° 0
*-base 0       = refl 0
*-base (suc x) =
   suc x * 0 ‚â°‚ü® refl _ ‚ü©
   x * 0 + 0 ‚â°‚ü® ap (_+ 0) (*-base x) ‚ü©
   0 + 0     ‚â°‚ü® refl _ ‚ü©
   0 ‚àé

*-comm : (x y : ‚Ñï) ‚Üí x * y ‚â° y * x
*-comm 0       y = sym (*-base y)
*-comm (suc x) y =
   suc x * y     ‚â°‚ü® refl _ ‚ü©
   x * y + y     ‚â°‚ü® +-comm (x * y) y ‚ü©
   y + x * y     ‚â°‚ü® ap (y +_) (*-comm x y) ‚ü©
   y + y * x     ‚â°‚ü® ap (_+ (y * x)) (sym (1-*-right-neutral y)) ‚ü©
   y * 1 + y * x ‚â°‚ü® sym (*-+-distrib y 1 x) ‚ü©
   y * (1 + x)   ‚â°‚ü® refl _ ‚ü©
   y * suc x     ‚àé

```

## Associativity of multiplication

```agda
*-assoc : (x y z : ‚Ñï) ‚Üí (x * y) * z ‚â° x * (y * z)
*-assoc zero    y z = refl _
*-assoc (suc x) y z = (x * y + y) * z     ‚â°‚ü® *-comm (x * y + y) z             ‚ü©
                      z * (x * y + y)     ‚â°‚ü® *-+-distrib z (x * y) y          ‚ü©
                      z * (x * y) + z * y ‚â°‚ü® ap (z * x * y +_) (*-comm z y)   ‚ü©
                      z * (x * y) + y * z ‚â°‚ü® ap (_+ y * z) (*-comm z (x * y)) ‚ü©
                      (x * y) * z + y * z ‚â°‚ü® ap (_+ y * z) (*-assoc x y z)    ‚ü©
                      x * y * z + y * z   ‚àé
```


## Even and odd numbers

```agda
is-even is-odd : ‚Ñï ‚Üí Type
is-even x = Œ£ y Íûâ ‚Ñï , x ‚â° 2 * y
is-odd  x = Œ£ y Íûâ ‚Ñï , x ‚â° 1 + 2 * y

zero-is-even : is-even 0
zero-is-even = 0 , refl 0

ten-is-even : is-even 10
ten-is-even = 5 , refl _

zero-is-not-odd : ¬¨ is-odd 0
zero-is-not-odd ()

one-is-not-even : ¬¨ is-even 1
one-is-not-even (0 , ())
one-is-not-even (suc (suc x) , ())

one-is-not-even' : ¬¨ is-even 1
one-is-not-even' (suc zero , ())

one-is-odd : is-odd 1
one-is-odd = 0 , refl 1

even-gives-odd-suc : (x : ‚Ñï) ‚Üí is-even x ‚Üí is-odd (suc x)
even-gives-odd-suc x (y , e) = goal
 where
  e' : suc x ‚â° 1 + 2 * y
  e' = ap suc e

  goal : is-odd (suc x)
  goal = y , e'

even-gives-odd-suc' : (x : ‚Ñï) ‚Üí is-even x ‚Üí is-odd (suc x)
even-gives-odd-suc' x (y , e) = y , ap suc e

odd-gives-even-suc : (x : ‚Ñï) ‚Üí is-odd x ‚Üí is-even (suc x)
odd-gives-even-suc x (y , e) = goal
 where
  y' : ‚Ñï
  y' = 1 + y

  e' : suc x ‚â° 2 * y'
  e' = suc x           ‚â°‚ü® ap suc e ‚ü©
       suc (1 + 2 * y) ‚â°‚ü® refl _ ‚ü©
       2 + 2 * y       ‚â°‚ü® sym (*-+-distrib 2 1 y) ‚ü©
       2 * (1 + y)     ‚â°‚ü® refl _ ‚ü©
       2 * y'          ‚àé

  goal : is-even (suc x)
  goal = y' , e'

even-or-odd : (x : ‚Ñï) ‚Üí is-even x ‚àî is-odd x
even-or-odd 0       = inl (0 , refl 0)
even-or-odd (suc x) = goal
 where
  IH : is-even x ‚àî is-odd x
  IH = even-or-odd x

  f : is-even x ‚àî is-odd x ‚Üí is-even (suc x) ‚àî is-odd (suc x)
  f (inl e) = inr (even-gives-odd-suc x e)
  f (inr o) = inl (odd-gives-even-suc x o)

  goal : is-even (suc x) ‚àî is-odd (suc x)
  goal = f IH
```

```agda
even : ‚Ñï ‚Üí Bool
even 0       = true
even (suc x) = not (even x)

even-true  : (y : ‚Ñï)  ‚Üí even (2 * y) ‚â° true
even-true 0       = refl _
even-true (suc y) = even (2 * suc y)         ‚â°‚ü® refl _ ‚ü©
                    even (suc y + suc y)     ‚â°‚ü® refl _ ‚ü©
                    even (suc (y + suc y))   ‚â°‚ü® refl _ ‚ü©
                    not (even (y + suc y))   ‚â°‚ü® ap (not ‚àò even) (+-step y y) ‚ü©
                    not (even (suc (y + y))) ‚â°‚ü® refl _ ‚ü©
                    not (not (even (y + y))) ‚â°‚ü® not-is-involution (even (y + y)) ‚ü©
                    even (y + y)             ‚â°‚ü® refl _ ‚ü©
                    even (2 * y)             ‚â°‚ü® even-true y ‚ü©
                    true ‚àé

even-false : (y : ‚Ñï) ‚Üí even (1 + 2 * y) ‚â° false
even-false 0       = refl _
even-false (suc y) = even (1 + 2 * suc y)   ‚â°‚ü® refl _ ‚ü©
                     even (suc (2 * suc y)) ‚â°‚ü® refl _ ‚ü©
                     not (even (2 * suc y)) ‚â°‚ü® ap not (even-true (suc y)) ‚ü©
                     not true               ‚â°‚ü® refl _ ‚ü©
                     false                  ‚àé

div-by-2 : ‚Ñï ‚Üí ‚Ñï
div-by-2 x = f (even-or-odd x)
 where
  f : is-even x ‚àî is-odd x ‚Üí ‚Ñï
  f (inl (y , _)) = y
  f (inr (y , _)) = y

even-odd-lemma : (y z : ‚Ñï) ‚Üí  1 + 2 * y ‚â° 2 * z ‚Üí ùüò
even-odd-lemma y z e = false-is-not-true impossible
 where
  impossible = false            ‚â°‚ü® sym (even-false y) ‚ü©
               even (1 + 2 * y) ‚â°‚ü® ap even e ‚ü©
               even (2 * z)     ‚â°‚ü® even-true z ‚ü©
               true             ‚àé

not-both-even-and-odd : (x : ‚Ñï) ‚Üí ¬¨ (is-even x √ó is-odd x)
not-both-even-and-odd x ((y , e) , (y' , o)) = even-odd-lemma y' y d
 where
  d = 1 + 2 * y' ‚â°‚ü® sym o ‚ü©
      x          ‚â°‚ü® e ‚ü©
      2 * y      ‚àé

double : ‚Ñï ‚Üí ‚Ñï
double 0 = 0
double (suc x) = suc (suc (double x))

double-correct : (x : ‚Ñï) ‚Üí double x ‚â° x + x
double-correct 0       = double 0 ‚â°‚ü® refl _ ‚ü©
                         0        ‚â°‚ü® refl _ ‚ü©
                         0 + 0    ‚àé
double-correct (suc x) = goal
 where
  IH : double x ‚â° x + x
  IH = double-correct x

  goal : double (suc x) ‚â° suc x + suc x
  goal = double (suc x)       ‚â°‚ü® refl _ ‚ü©
         suc (suc (double x)) ‚â°‚ü® ap (suc ‚àò suc) IH ‚ü©
         suc (suc (x + x))    ‚â°‚ü® ap suc (sym (+-step x x)) ‚ü©
         suc (x + suc x)      ‚â°‚ü® refl _ ‚ü©
         suc x + suc x        ‚àé
```
