```agda
{-# OPTIONS --without-K --safe #-}

module lecture3 where

-- lecture 3
-- Plan: Complete last lecture.
--       Generalize some definitions to use universe levels.
--       Uses of Sigma, including examples like monoids.
--       Use of universes to prove that Â¬ (false â‰¡ true).
--       Characterization of equality in Î£ types.


open import lecture1 hiding (ğŸ˜ ; ğŸ™ ; â‹† ; D ; _â‰£_)
open import lecture2 using (is-prime ; _*_ ; ğŸ˜ ; ğŸ™ ; â‹† ; _â‰¥_)

-- Give Î£ a universe-polymorphic type

open import Agda.Primitive using (Level; lzero; lsuc; _âŠ”_)
                           renaming (Set to ğ“¤)
                           public

variable i j k : Level

record Î£ {A : ğ“¤ i} (B : A â†’ ğ“¤ j) : ğ“¤ (i âŠ” j) where
 constructor
  _,_
 field
  prâ‚ : A
  prâ‚‚ : B prâ‚

open Î£ public
infixr 1 _,_

Sigma : (A : ğ“¤ i) (B : A â†’ ğ“¤ j) â†’ ğ“¤ (i âŠ” j)
Sigma {i} {j} A B = Î£ {i} {j} {A} B

syntax Sigma A (Î» x â†’ b) = Î£ x ê‰ A , b

infix -1 Sigma

_Ã—_ : ğ“¤ i â†’ ğ“¤ j â†’ ğ“¤ (i âŠ” j)
A Ã— B = Î£ x ê‰ A , B

-- (x : X) â†’ A x
-- (x : X) Ã— A x

infixr 2 _Ã—_

-- More general type of negation:

Â¬_ : ğ“¤ i â†’ ğ“¤ i
Â¬ A = A â†’ ğŸ˜

-- Give the identity type more general universe assignments:

data _â‰¡_ {X : ğ“¤ i} : X â†’ X â†’ ğ“¤ i where
 refl : (x : X) â†’ x â‰¡ x

_â‰¢_ : {X : ğ“¤ i} â†’ X â†’ X â†’ ğ“¤ i
x â‰¢ y = Â¬ (x â‰¡ y)

infix 0 _â‰¡_

â‰¡-elim : {X : ğ“¤ i} (A : (x y : X) â†’ x â‰¡ y â†’ ğ“¤ j)
       â†’ ((x : X) â†’ A x x (refl x))
       â†’ (x y : X) (p : x â‰¡ y) â†’ A x y p
â‰¡-elim A f x x (refl x) = f x

â‰¡-nondep-elim : {X : ğ“¤ i} (A : X â†’ X â†’ ğ“¤ j)
              â†’ ((x : X) â†’ A x x)
              â†’ (x y : X) â†’ x â‰¡ y â†’ A x y
â‰¡-nondep-elim A = â‰¡-elim (Î» x y _ â†’ A x y)

trans : {A : ğ“¤ i} {x y z : A} â†’ x â‰¡ y â†’ y â‰¡ z â†’ x â‰¡ z
trans p (refl y) = p

sym : {A : ğ“¤ i} {x y : A} â†’ x â‰¡ y â†’ y â‰¡ x
sym (refl x) = refl x

ap : {A : ğ“¤ i} {B : ğ“¤ j} (f : A â†’ B) {x y : A} â†’ x â‰¡ y â†’ f x â‰¡ f y
ap f (refl x) = refl (f x)

apâ‚‚ : {A : ğ“¤ i} {B : ğ“¤ j} {C : ğ“¤ k} (f : A â†’ B â†’ C) {x x' : A} {y y' : B}
    â†’ x â‰¡ x' â†’ y â‰¡ y' â†’ f x y â‰¡ f x' y'
apâ‚‚ f (refl x) (refl y) = refl (f x y)

transport : {X : ğ“¤ i} (A : X â†’ ğ“¤ j)
          â†’ {x y : X} â†’ x â‰¡ y â†’ A x â†’ A y
transport A (refl x) a = a

_âˆ™_ : {A : ğ“¤ i} {x y z : A} â†’ x â‰¡ y â†’ y â‰¡ z â†’ x â‰¡ z
_âˆ™_ = trans

infixl 7 _âˆ™_

_â»Â¹ : {A : ğ“¤ i} {x y : A} â†’ x â‰¡ y â†’ y â‰¡ x
_â»Â¹ = sym

infix  40 _â»Â¹

-- The (sub)type of prime numbers

â„™ : ğ“¤â‚€
â„™ = Î£ p ê‰ â„• , is-prime p

â„™-inclusion : â„™ â†’ â„•
â„™-inclusion = prâ‚

-- We can prove that this map is left-cancellable, i.e. it satisfies
-- â„™-inclusion u â‰¡ â„™-inclusion u â†’ u â‰¡ v.
-- Moreover, this map is an embedding (we haven't defined this concept yet).

-- Not quite the type of composite numbers:

CN : ğ“¤
CN = Î£ x ê‰ â„• , Î£ (y , z) ê‰ â„• Ã— â„• , x â‰¡ y * z

CN' : ğ“¤
CN' = Î£ x ê‰ â„• , Î£ (y , z) ê‰ â„• Ã— â„• , (y â‰¥ 2) Ã— (z â‰¥ 2) Ã— (x â‰¡ y * z)

CN-projection : CN â†’ â„•
CN-projection = prâ‚

-- This map is not left-cancellable, and hence can't be considered to
-- be an an inclusion.

counter-example : CN-projection (6 , (3 , 2) , refl 6)
                â‰¡ CN-projection (6 , (2 , 3) , refl 6)
counter-example = refl 6

-- But how do we prove that these two tuples are *different*? They
-- certainly do look different. We'll do this later.

-- We will need to define
--
-- CN = Î£ x ê‰ â„• , âˆ¥ Î£ (y , z) ê‰ â„• Ã— â„• , x â‰¡ y * z âˆ¥, or equivalently
-- CN = Î£ x ê‰ â„• , âˆƒ (y , z) ê‰ â„• Ã— â„• , x â‰¡ y * z âˆ¥
--
-- to really get a *subtype* of composite numbers.


-- Another use of Î£.
-- The type of monoids.

is-prop : ğ“¤ i â†’ ğ“¤ i
is-prop X = (x y : X) â†’ x â‰¡ y

is-set : ğ“¤ i â†’ ğ“¤ i
is-set X = (x y : X) â†’ is-prop (x â‰¡ y)

Mon : ğ“¤ (lsuc i)
Mon {i} = Î£ X ê‰ ğ“¤ i  -- data
            , is-set X  -- property (we show that)
            Ã— (Î£ ğŸ ê‰ X ,  -- data (but...)
               Î£ _Â·_ ê‰ (X â†’ X â†’ X) -- data
                  , (((x : X) â†’ (x Â· ğŸ â‰¡ x)) -- (1) property
                  Ã—  ((x : X) â†’ (ğŸ Â· x â‰¡ x)) -- (2) property
                  Ã—  ((x y z : X) â†’ (x Â· (y Â· z)) â‰¡ ((x Â· y) Â· z)))) -- (3) property

-- This can be defined using a record in Agda:

record Mon' : ğ“¤ (lsuc i) where
 constructor mon
 field
  carrier        : ğ“¤ i  -- X
  carrier-is-set : is-set carrier
  ğŸ              : carrier
  _Â·_            : carrier â†’ carrier â†’ carrier
  left-unit-law  : (x : carrier) â†’ x Â· ğŸ â‰¡ x
  right-unit-law : (x : carrier) â†’ ğŸ Â· x â‰¡ x
  assoc-law      : (x y z : carrier) â†’ (x Â· (y Â· z)) â‰¡ ((x Â· y) Â· z)

Î± : Mon {i} â†’ Mon' {i}
Î± (X , X-is-set , ğŸ , _Â·_ , l , r , a) = mon X X-is-set ğŸ _Â·_ l r a

Î² : Mon' {i} â†’ Mon {i}
Î² (mon X X-is-set ğŸ _Â·_ l r a) = (X , X-is-set , ğŸ , _Â·_ , l , r , a)

Î²Î± : (M : Mon {i}) â†’ Î² (Î± M) â‰¡ M
Î²Î± = refl

Î±Î² : (M : Mon' {i}) â†’ Î± (Î² M) â‰¡ M
Î±Î² = refl

-- This kind of proof doesn't belong to the realm of MLTT:

false-is-not-true[not-an-MLTT-proof] : false â‰¢ true
false-is-not-true[not-an-MLTT-proof] ()

-- Proof in MLTT, which requires a universe (Cf. Ulrik's 2nd HoTT
-- lecture):

_â‰£_ : Bool â†’ Bool â†’ ğ“¤â‚€
true  â‰£ true  = ğŸ™
true  â‰£ false = ğŸ˜
false â‰£ true  = ğŸ˜
false â‰£ false = ğŸ™

â‰¡-gives-â‰£ : {x y : Bool} â†’ x â‰¡ y â†’ x â‰£ y
â‰¡-gives-â‰£ (refl true)  = â‹†
â‰¡-gives-â‰£ (refl false) = â‹†

false-is-not-true : Â¬ (false â‰¡ true)
false-is-not-true p = II
 where
  I : false â‰£ true
  I = â‰¡-gives-â‰£ p

  II : ğŸ˜
  II = I

false-is-not-true' : Â¬ (false â‰¡ true)
false-is-not-true' = â‰¡-gives-â‰£

-- Notice that this proof is different from the one given by Ulrik in
-- the HoTT track. Exercise: implement Ulrik's proof in Agda.

-- Exercise: prove that Â¬ (0 â‰¡ 1) in the natural numbers in MLTT style
-- without using `()`.

-- contrapositives.

contrapositive : {A : ğ“¤ i} {B : ğ“¤ j} â†’ (A â†’ B) â†’ (Â¬ B â†’ Â¬ A)
contrapositive f g a = g (f a)

Î -Â¬-gives-Â¬-Î£ : {X : ğ“¤ i} {A : X â†’ ğ“¤ j}
              â†’ ((x : X) â†’ Â¬ A x)
              â†’ Â¬ (Î£ x ê‰ X , A x)
Î -Â¬-gives-Â¬-Î£ Ï• (x , a) = Ï• x a

Â¬-Î£-gives-Î -Â¬ : {X : ğ“¤ i} {A : X â†’ ğ“¤ j}
              â†’ Â¬ (Î£ x ê‰ X , A x)
              â†’ ((x : X) â†’ Â¬ A x)
Â¬-Î£-gives-Î -Â¬ Î³ x a = Î³ (x , a)


-- Equality in Î£ types.

from-Î£-â‰¡' : {X : ğ“¤ i} {A : X â†’ ğ“¤ j}
            {(x , a) (y , b) : Î£ A}
          â†’ (x , a) â‰¡ (y , b)
          â†’ Î£ p ê‰ (x â‰¡ y) , (transport A p a â‰¡ b)
from-Î£-â‰¡' (refl (x , a)) = (refl x , refl a)

to-Î£-â‰¡' : {X : ğ“¤ i} {A : X â†’ ğ“¤ j}
          {(x , a) (y , b) : Î£ A}
        â†’ (Î£ p ê‰ (x â‰¡ y) , (transport A p a â‰¡ b))
        â†’ (x , a) â‰¡ (y , b)
to-Î£-â‰¡' (refl x , refl a) = refl (x , a)

module _ {X : ğ“¤ i} {A : ğ“¤ j}
         {(x , a) (y , b) : X Ã— A} where

 from-Ã—-â‰¡ : (x , a) â‰¡ (y , b)
          â†’ (x â‰¡ y) Ã— (a â‰¡ b)
 from-Ã—-â‰¡ (refl (x , a)) = refl x , refl a


 to-Ã—-â‰¡ : (x â‰¡ y) Ã— (a â‰¡ b)
        â†’ (x , a) â‰¡ (y , b)
 to-Ã—-â‰¡ (refl x , refl a) = refl (x , a)

module _ {X : ğ“¤ i} {A : X â†’ ğ“¤ j}
         {(x , a) (y , b) : Î£ A} where

 -- x y : X
 -- a : A x
 -- b : A y

 from-Î£-â‰¡ : (x , a) â‰¡ (y , b)
          â†’ Î£ p ê‰ (x â‰¡ y) , transport A p a â‰¡ b
 from-Î£-â‰¡ (refl (x , a)) = refl x , refl a


 to-Î£-â‰¡ : (Î£ p ê‰ (x â‰¡ y) , (transport A p a â‰¡ b))
        â†’ (x , a) â‰¡ (y , b)
 to-Î£-â‰¡ (refl x , refl a) = refl (x , a)


 contra-from-Î£-â‰¡ : Â¬ (Î£ p ê‰ (x â‰¡ y) , (transport A p a â‰¡ b))
                 â†’ (x , a) â‰¢ (y , b)
 contra-from-Î£-â‰¡ = contrapositive from-Î£-â‰¡

 contra-to-Î£-â‰¡ : (x , a) â‰¢ (y , b)
               â†’ Â¬ (Î£ p ê‰ (x â‰¡ y) , (transport A p a â‰¡ b))
 contra-to-Î£-â‰¡ = contrapositive to-Î£-â‰¡

 to-Î£-â‰¢ : ((p : x â‰¡ y) â†’ transport A p a â‰¢ b)
        â†’ (x , a) â‰¢ (y , b)
 to-Î£-â‰¢ u = contra-from-Î£-â‰¡ (Î -Â¬-gives-Â¬-Î£ u)

 from-Î£-â‰¢ : (x , a) â‰¢ (y , b)
          â†’ ((p : x â‰¡ y) â†’ transport A p a â‰¢ b)
 from-Î£-â‰¢ v = Â¬-Î£-gives-Î -Â¬ (contra-to-Î£-â‰¡ v)
```

We now revisit the example above. How do we prove that aa and bb are
different? It's not easy. We use the above lemmas.

```agda
aa bb : CN
aa = (6 , (3 , 2) , refl 6)
bb = (6 , (2 , 3) , refl 6)
```

To prove that aa â‰¢ bb, we need to know that â„• is a set! And this is
difficult. See the module
[Hedbergs-Theorem](../Lecture-Notes/Hedbergs-Theorem.lagda.md) for a
complete proof.

For the moment we just assume that â„• is a set, and prove that 3 â‰¢ 2 by
cheating (produce a genuine MLTT proof as an exercise).

```agda

3-is-not-2 : 3 â‰¢ 2
3-is-not-2 ()

example-revisited : is-set â„• â†’ aa â‰¢ bb
example-revisited â„•-is-set = I
 where
  A : â„• â†’ ğ“¤â‚€
  A x = Î£ (y , z) ê‰ â„• Ã— â„• , x â‰¡ y * z

  II : (p : 6 â‰¡ 6) â†’ transport A p ((3 , 2) , refl 6) â‰¢  ((2 , 3) , refl 6)
  II p = VIII
   where
    III : p â‰¡ refl 6
    III = â„•-is-set 6 6 p (refl 6)

    IV : transport A p ((3 , 2) , refl 6) â‰¡ ((3 , 2) , refl 6)
    IV = ap (Î» - â†’ transport A - ((3 , 2) , refl 6)) III

    V : ((3 , 2) , refl 6) â‰¢ ((2 , 3) , refl 6)
    V q = 3-is-not-2 VII
     where
      VI : (3 , 2) â‰¡ (2 , 3)
      VI = ap prâ‚ q

      VII : 3 â‰¡ 2
      VII = ap prâ‚ VI

    VIII : transport A p ((3 , 2) , refl 6) â‰¢  ((2 , 3) , refl 6)
    VIII r = V IX
     where
      IX : ((3 , 2) , refl 6) â‰¡ ((2 , 3) , refl 6)
      IX = trans (IV â»Â¹) r

  I : aa â‰¢ bb
  I = to-Î£-â‰¢ II
```

If there is time, I will do some isomorphisms.
